\begin{eqnarray}
  & & \frac{d\sigma_{\pi^-\Sigma^+}}{dM d\Omega}
  = \frac{1}{3} A_{I=0} |T_{I=0}|^2 + \frac{1}{2} A_{I=1} |T_{I=1}|^2 + \frac{2}{\sqrt{6}} \sqrt{A_{I=0} A_{I=1}} \mbox{\bf Re}(T_{I=0}T_{I=1}^*) \nonumber \\
  & & \frac{d\sigma_{\pi^+\Sigma^-}}{dM d\Omega}
  = \frac{1}{3} A_{I=0} |T_{I=0}|^2 + \frac{1}{2} A_{I=1} |T_{I=1}|^2 - \frac{2}{\sqrt{6}} \sqrt{A_{I=0} A_{I=1}} \mbox{\bf Re}(T_{I=0}T_{I=1}^*) \nonumber \\
  & & \frac{d\sigma_{\pi^0\Sigma^-}}{dM d\Omega}  =  \frac{1}{2} A_{I=1} |T_{I=1}|^2 \nonumber \\
  \label{eq::CS_iso_wA}
\end{eqnarray}
